added Gcounter and Account

consys-invariants/invariants-lang/test.dfy
@@ -52,12 +52,37 @@ function method replica(): int
     42
 }
 
+
+function sum(s: set<int>): int
+{
+    var v :| v in s; v + (sum(s - { v }))
+}
+
+
+
 class GCounter {
     var increments: map<int, int>;
 
-    constructor() 
+
+    predicate isWellformed()
+        reads this; 
+    {
+        (forall i :: i in increments.Keys ==> increments[i] >= 0) && replicas() == increments.Keys
+    }
+
+    
+
+    constructor(incs: map<int, int>)
+        requires forall i :: i in incs.Keys ==> incs[i] >= 0;
+        requires replicas() == incs.Keys;
+        ensures isWellformed();
+    {
+        this.increments := incs;
+    }
+
+    constructor Zero() 
         ensures forall i :: i in increments.Keys ==> increments[i] == 0;
-        ensures replicas() == increments.Keys;
+        ensures isWellformed();
     {
         var incs: map<int, int> := map[];
 
@@ -75,16 +100,17 @@ class GCounter {
         increments := incs;
     }
 
-
+    
     method GetValue() returns (result: int)
-        requires forall i :: i in increments.Keys ==> increments[i] >= 0; 
-        ensures forall i :: i in increments.Keys ==> increments[i] >= 0;
-        ensures result >= 0; 
+        requires isWellformed();
+        ensures result >= 0;
+        ensures result == sum(increments.Values);
     {
         var values := increments.Values;
         var sum := 0;
 
         while ( values != {} )
+            invariant forall v :: v in values ==> v >= 0;
             invariant sum >= 0;
             decreases values;
         {
@@ -97,33 +123,131 @@ class GCounter {
     }
 
 
-    method Inc() 
-        requires forall i :: i in increments ==> increments[i] >= 0; 
-        requires replicas() == increments.Keys;
-        ensures forall i :: i in increments ==> increments[i] >= 0;
-        ensures replicas() == increments.Keys;
+    method Inc(n: int) 
+        requires n >= 0;
+        requires isWellformed();
+        ensures isWellformed();
         modifies this;
     {
         var v := increments[replica()];
-        increments := increments + map[replica() := v + 1];
+        increments := increments + map[replica() := v + n];
     }
 
 
     method Merge(other: GCounter) returns (result: GCounter)
-        requires forall i :: i in increments ==> increments[i] >= 0; 
-        requires replicas() == increments.Keys;
-        ensures forall i :: i in increments ==> increments[i] >= 0;
-        ensures replicas() == increments.Keys;
+        requires isWellformed();
+        requires other.isWellformed();
+        ensures result.isWellformed();
     {
-        
+        var incs: map<int, int> := map[];
+
+        var rs := replicas(); 
+
+        while (rs != {})
+            invariant forall i :: i in incs.Keys ==> incs[i] >= 0;
+            invariant replicas() == rs + incs.Keys;
+            decreases rs;
+        {
+            var r :| r in rs;
+            var thisV := increments[r];
+            var otherV := other.increments[r];
+
+            incs := incs + map[r := thisV + otherV];
+            rs := rs - {r};
+        }        
+        return new GCounter(incs);                
+    }
+}
+
+
+class Account {
+    var deposits: GCounter;
+    var withdraws: GCounter;
+
+    predicate isWellformed()
+        reads this;
+        reads deposits;
+        reads withdraws; 
+    {
+        deposits.isWellformed() && withdraws.isWellformed()
     }
 
+    constructor(deposits: GCounter, withdraws: GCounter) 
+        requires deposits.isWellformed();
+        requires withdraws.isWellformed();
+        ensures isWellformed();
+    {
+        this.deposits := deposits;
+        this.withdraws := withdraws;        
+    }
+
+    constructor Zero() 
+        ensures isWellformed();
+    {
+        this.deposits := new GCounter.Zero();
+        this.withdraws := new GCounter.Zero();
+    }
+
+    method GetValue() returns (result: int)
+        ensures result == sum(deposits.increments.Values) - sum(withdraws.increments.Values);
+    {
+        var plus := deposits.GetValue();
+        var minus := withdraws.GetValue();
+        return plus - minus;
+    }
+
+    method Deposit(n: int)
+        requires n >= 0;
+        requires isWellformed();
+        ensures isWellformed();
+        modifies deposits;
+    {
+        deposits.Inc(n);
+    }
+
+    method Withdraw(n: int)
+        requires n >= 0;
+        requires isWellformed();
+        ensures isWellformed();
+        modifies withdraws;
+    {
+        withdraws.Inc(n);
+    }
+
+    method Merge(other: Account) returns (result: Account)
+        requires isWellformed();
+        requires other.isWellformed();
+        ensures result.isWellformed();
+    {
+        var newDeposits := deposits.Merge(other.deposits);
+        var newWithdraws := withdraws.Merge(other.withdraws);
+
+        return new Account(newDeposits, newWithdraws);
+    }
+    
+
+}
 
 
+
+method AccountTest(acc1: Account, acc2 : Account) 
+    requires acc1.isWellformed();
+    requires acc2.isWellformed();
+    modifies acc1, acc2, acc1.deposits, acc2.deposits, acc1.withdraws, acc2.withdraws;
+{
+    var a := acc1;
+    var b := acc2;
+    
+    a.Deposit(500);
+    a.Deposit(100);
+
+    b.Deposit(200);
+
+    a := a.Merge(b);
+    b := b.Merge(a);
 
 
 
 
 }
-
 
